There are major 4 different forms in which equation of line can be represented are:-
1. Slope-Point Form
2. Two Point Form
3. Slope-Intercept Form
4. Intercept Form of Straight Line
# Slope-Point Form:
The equation of a straight line whose slope is $m$ and which passes through a point ($x_{1},y_{1}$) is found using the point-slope form. The equation of the point-slope form is,
$$
y-y_{1} = m(x-x_{1})
$$
Where, (x, y) is a arbitrary point on the line.

Let us see how to find the point-slope form. We will derive this formula using the equation for the slope of a line. Let us consider a line whose slope is m. Let us assume that ($x_{1},y_{1}$) is a known point on the line. Let ($x,y$) be any other random point on the line whose coordinates are not known. We know that the equation for the slope of a line is:
$$
\text{Slope(m) =} \frac{\text{Difference in y-coordinate}}{\text{Difference in x-coordinate}} = \frac{y-y_{1}}{x-x_{1}}
$$
Multiplying both side by $(x- x_{1})$
$$
m(x-x_{1}) = (y-y_{1})
$$
This can be written as,
$$
y-y_{1} = m(x-x_{1})
$$
Hence, Proved.

# Two Point Form:
Consider a line with two points $(x_{1},y_{1})$ and $(x_{2},y_{2})$ on it. Then its slope can be calculated by the formula of Slope. Substituting this in the [Slope-Point Form](Slope-Point%20Form.md), we get the two point form as, 
$$
y-y_{1} = \frac{(y_{2}-y_{1})}{(x_{2}-x_{1})}
$$

# Slope-Intercept Form:
Suppose a line is given to you with its slope $m$ and its y-intercept. Say, a line intersects the y-axis at the point (0, c). Using the [Slope-Point Form](Slope-Point%20Form.md) we have, 
$$
y-c= m(x-0) \implies y = mx + c
$$ 
where, $c$ is the y-intercept. This is called slope-intercept form of a line.

**Note:** If d is the x-intercept, then the slope-intercept form of the equation of the line is $y = m(x-d)$.

# Intercept Form:
If (a, 0) and (0, b) are the x and y intercepts of a line respectively. Then its slope is,
$$
m = \frac{b-0}{(0-a)} =-\frac{b}{a}
$$
Then, its equation using the [Slope-Point Form](Slope-Point%20Form.md) is,
$$
y-0 =-\frac{b}{a}(x-a)
$$
Multiplying both side by $a$,
$$
ay =-bx + ab
$$
$$
bx + ay = ab
$$
Dividing both sides by ab,
$$
\frac{x}{a} + \frac{y}{b}= 1
$$

